Finish proof kvs_read

theories/case_studies/multiuser_kvs/kvs_spec.v
@@ -12,8 +12,6 @@ Class kvsG Σ :=
       kvs_genG :: gen_heapGS nat kvs_entry Σ; (* memory *)
     }.
 
-(* Notation "r ↦ᵣ{ q } w" := (pointsto (L:=RegName) (V:=Word) r q w) *)
-
 Definition kvs_frag_idx_frac `{kvsG} (idx : nat) (k : Z) (w : Word) (q : dfrac) : iProp Σ :=
   (pointsto (L:=nat) (V:=kvs_entry) idx q (k,w)).
 Notation "k '⤇(KVS){' q '}[' idx  ']' w" :=
@@ -23,8 +21,6 @@ Notation "k '⤇(KVS)[' idx  ']' w" :=
 
 Definition kvs_frag `{kvsG} (k : Z ) (w : Word) : iProp Σ := ∃ idx, k ⤇(KVS)[ idx ] w.
 Notation "k '⤇(KVS)' w" := (kvs_frag k w) (at level 20) : bi_scope.
-(* Global Instance persistent_kvs_frag k w : Persistent (k ⤇(KVS) w)%I. *)
-(* Admitted. *)
 
 Notation "●(KVS) m" := (gen_heap_interp m) (at level 20) : bi_scope.
 
@@ -43,19 +39,22 @@ Section KVS_spec.
   Definition isKVS_entry (a : Addr) (idx : nat) (kw : Z * Word) : iProp Σ :=
     (a ^+ (2*idx))%a ↦ₐ (WInt kw.1) ∗ (a ^+ (2*idx + 1))%a ↦ₐ kw.2.
 
-  Definition kvs_dom : gset nat := list_to_set (seq 0 (SIZE_MAP -1)).
+  Definition kvs_dom : gset nat := set_seq 0 SIZE_MAP.
+
+  Definition wf_kvs_map (m : kvs_map) : Prop :=
+    dom m = kvs_dom ∧ NoDup (fst <$> (snd <$> (map_to_list m))).
 
   Definition isKVS
     (a : Addr) (m : kvs_map) : iProp Σ :=
-    ⌜ dom m = kvs_dom⌝ ∗
+    ⌜ wf_kvs_map m ⌝ ∗
     ●(KVS) m ∗
     [∗ map] idx ↦ kw ∈ m, isKVS_entry a idx kw.
 
   Definition isKVS_open
-    (a : Addr) (m : kvs_map) (open_idx : Z) : iProp Σ :=
-    ⌜ dom m = kvs_dom⌝ ∗
+    (a : Addr) (m : kvs_map) (open_idx : nat) : iProp Σ :=
+    ⌜ wf_kvs_map m ⌝ ∗
     ●(KVS) m ∗
-    [∗ map] idx ↦ kw ∈ m, if (decide (Z.of_nat idx = open_idx)%Z) then True else isKVS_entry a idx kw.
+    [∗ map] idx ↦ kw ∈ (delete open_idx m), isKVS_entry a idx kw.
 
 
   Lemma kvs_frag_kvs_frag_idx (k : Z) (w : Word) :
@@ -76,23 +75,10 @@ Section KVS_spec.
     k ⤇(KVS)[idx] w.
   Proof.
     iIntros "( (%HdomKVS & Hkvs_auth & HKVS) & Hk)".
-  Admitted.
-
-  Lemma open_isKVS_kvs_frag
-    (b : Addr) (m : kvs_map)
-    (k : Z ) (w : Word) :
-    isKVS b m ∗
-    k ⤇(KVS) w -∗
-    ∃ idx : nat,
-      isKVS_open b m idx ∗
-      isKVS_entry b idx (k, w) ∗
-      k ⤇(KVS) w.
-  Proof.
-    iIntros "(HKVS & Hkvs_frag)".
-    iDestruct (kvs_frag_kvs_frag_idx with "Hkvs_frag") as (idx) "Hkvs_frag".
-    iExists idx.
-    iDestruct (open_isKVS_kvs_frag_idx with "[$HKVS $Hkvs_frag]") as "($ & $ & Hkvk_frag)".
-    by iApply kvs_frag_idx_kvs_frag.
+    iDestruct (gen_heap_valid with "Hkvs_auth Hk") as "%Hidx'".
+    rewrite -{2}(insert_id m idx (k,w)); last done.
+    iDestruct (big_sepM_insert_delete with "HKVS") as "[Hkvs_entry HKVS]".
+    iFrame; eauto.
   Qed.
 
   Lemma close_isKVS_kvs_frag_idx
@@ -105,7 +91,60 @@ Section KVS_spec.
     k ⤇(KVS)[ idx ] w
   .
   Proof.
-  Admitted.
+    iIntros "( (%HdomKVS & Hkvs_auth & HKVS) & Hkvs_entry & Hk)".
+    iDestruct (gen_heap_valid with "Hkvs_auth Hk") as "%Hidx'".
+    iDestruct (big_sepM_delete with "[$HKVS $Hkvs_entry]") as "HKVS"; eauto.
+    iFrame; eauto.
+  Qed.
+
+  Lemma open_isKVS_kvs_frag_idx_diff
+    (b : Addr) (m : kvs_map) (idx idx' : nat) (k : Z) (w : Word):
+    0 <= idx' < SIZE_MAP ->
+    idx ≠ idx' ->
+    isKVS b m ∗
+    k ⤇(KVS)[ idx ] w -∗
+    ∃ k' w',
+      ⌜ k ≠ k' ⌝ ∗ ⌜ m !! idx' = Some (k', w') ⌝ ∗
+      isKVS_open b m idx' ∗
+      k ⤇(KVS)[ idx ] w ∗
+      isKVS_entry b idx' (k', w').
+  Proof.
+    iIntros (Hidx' Hidx) "( (%Hwf & Hkvs_auth & HKVS) & Hk)".
+    destruct Hwf as [Hkvs_dom Hkvs_uniqueness].
+    iDestruct (gen_heap_valid with "Hkvs_auth Hk") as "%Hm_idx".
+    assert (is_Some (m !! idx')) as [ [k' w'] Hm_idx'].
+    { apply elem_of_dom. rewrite Hkvs_dom /kvs_dom.
+      by apply elem_of_set_seq.
+    }
+    assert (k ≠ k') as Hkk'.
+    { rewrite -(insert_id m idx (k, w)) in Hkvs_uniqueness; last done.
+      rewrite -insert_delete_eq in Hkvs_uniqueness.
+      rewrite -(insert_id (<[idx:=(k, w)]> (delete idx m)) idx' (k', w')) in Hkvs_uniqueness; last by simplify_map_eq.
+      rewrite -insert_delete_eq in Hkvs_uniqueness.
+      rewrite -(insert_delete_ne _ idx idx') in Hkvs_uniqueness; auto.
+      rewrite map_to_list_insert in Hkvs_uniqueness; last by simplify_map_eq.
+      rewrite map_to_list_insert in Hkvs_uniqueness; last by simplify_map_eq.
+      cbn in Hkvs_uniqueness.
+      apply NoDup_cons_1_1 in Hkvs_uniqueness.
+      set_solver+Hkvs_uniqueness.
+    }
+    iExists k',w'.
+    rewrite -{2}(insert_id m idx' (k',w')); last done.
+    iDestruct (big_sepM_insert_delete with "HKVS") as "[ [Hkb' Hkw'] HKVS]".
+    iFrame; eauto.
+  Qed.
+
+  Lemma close_isKVS
+    (b : Addr) (m : kvs_map) (idx : nat) (k : Z) (w : Word):
+    m !! idx = Some (k, w) ->
+    isKVS_open b m idx ∗
+    isKVS_entry b idx (k, w) -∗
+    isKVS b m.
+  Proof.
+    iIntros (Hidx) "[(%Hwf & Hkvs_auth & HKVS) Hkvs_entry]"; cbn.
+    iDestruct (big_sepM_delete with "[$HKVS $Hkvs_entry]") as "HKVS"; eauto.
+    iFrame; eauto.
+  Qed.
 
   (* TODO move *)
   Notation "r ↦ᵣ -" := (∃ w, pointsto (L:=RegName) (V:=Word) r (DfracOwn 1) w)%I (at level 20) : bi_scope.
@@ -182,75 +221,17 @@ Section KVS_spec.
     iApply "Hpost"; iFrame.
   Qed.
 
-
-  Lemma open_isKVS
-    (b : Addr) (m : kvs_map) (idx : Z):
-    (0 ≤ idx < 16)%Z ->
-    (* (e + 32)%a = Some b -> *)
-    isKVS b m -∗
-    ∃ ku kn w,
-      isKVS_open b m idx ∗
-      (b ^+ (2*idx))%a ↦ₐ WInt (kvs_full_key ku kn) ∗
-      (b ^+ (1+2*idx))%a ↦ₐ w.
-  Proof.
-    (*         generalize dependent b. *)
-    (*         induction idx; iIntros (b Hkvs_size Hidx) "HKVS"; cbn. *)
-    (*         - iDestruct "HKVS" as "%HKVS". solve_addr. *)
-    (*         - destruct a as [k w]; iDestruct "HKVS" as "(Hb & Hb' & HKVS)". *)
-    (*           destruct ((idx =? 0)%Z). *)
-    (*           + iExists (kvs_reverse_full_key k), w. *)
-    (*             admit. *)
-    (*           + iFrame. *)
-    (*             iDestruct (IHm with "HKVS") as "HKVS"; auto. *)
-    (* admit. *)
-    (*           exists k, w. *)
-  Admitted.
-
-  Lemma close_isKVS
-    (b : Addr) (m : kvs_map) (idx : Z) (ku kn : Z) (w : Word):
-    (0 ≤ idx < 16)%Z ->
-    (* (e + 32)%a = Some b -> *)
-    isKVS_open b m idx ∗
-    (b ^+ (2*idx))%a ↦ₐ WInt (kvs_full_key ku kn) ∗
-    (b ^+ (1+2*idx))%a ↦ₐ w -∗
-    isKVS b m.
-  Proof.
-    (*         generalize dependent b. *)
-    (*         induction idx; iIntros (b Hkvs_size Hidx) "HKVS"; cbn. *)
-    (*         - iDestruct "HKVS" as "%HKVS". solve_addr. *)
-    (*         - destruct a as [k w]; iDestruct "HKVS" as "(Hb & Hb' & HKVS)". *)
-    (*           destruct ((idx =? 0)%Z). *)
-    (*           + iExists (kvs_reverse_full_key k), w. *)
-    (*             admit. *)
-    (*           + iFrame. *)
-    (*             iDestruct (IHm with "HKVS") as "HKVS"; auto. *)
-    (* admit. *)
-    (*           exists k, w. *)
-  Admitted.
-
-  (* From cap_machine Require Import bitblast. *)
-  Lemma kvs_full_key_inj (uk1 nk1 uk2 nk2 : Z) :
-    (0 <= nk1 < 16)%Z ->
-    (0 <= nk2 < 16)%Z ->
-    (0 <= uk1)%Z ->
-    (0 <= uk2)%Z ->
-    (kvs_full_key uk1 nk1 = kvs_full_key uk2 nk2)%Z -> uk1 = uk2 ∧ nk1 = nk2.
-  Proof.
-    intros Hnk1 Hnk2 Huk1 Huk2 Heq.
-    rewrite /kvs_full_key in Heq.
-  Admitted.
-
   Lemma KVS_search_spec `{KVS : kvsLayout}
     (pc_b pc_e pc_a : Addr)
     (cgp_b cgp_e : Addr)
     (rkey ridx rscratch : RegName)
-    (user_key nkey : Z)
+    (fkey : Z)
     (m : kvs_map) (w : Word)
     :
     let instrs := (kvs_search_instrs rkey ridx rscratch) in
-    let fkey := (kvs_full_key user_key nkey) in
     SubBounds pc_b pc_e pc_a (pc_a ^+ length instrs)%a ->
     withinBounds cgp_b cgp_e cgp_b = true ->
+    ((cgp_b + (1 + 2*SIZE_MAP)%Z)%a = Some cgp_e)%a ->
 
     rscratch ≠ cnull ->
     ridx ≠ cnull ->
@@ -269,15 +250,15 @@ Section KVS_spec.
       codefrag pc_a instrs ∗
       ▷ ( ∀ idx,
             (
-              ⌜ (0 <= idx)%Z ⌝ ∗
+              ⌜ (0 <= idx) ⌝ ∗
               PC ↦ᵣ WCap RX Global pc_b pc_e (pc_a ^+ length instrs)%a ∗
               cgp ↦ᵣ WCap RW Global cgp_b cgp_e (cgp_b ^+ (1+2*idx) )%a ∗
               rkey ↦ᵣ WInt fkey ∗
               ridx ↦ᵣ WInt idx ∗
               rscratch ↦ᵣ - ∗
 
-              isKVS_open (cgp_b ^+ 1)%a  m idx ∗
-              (cgp_b ^+ (1+2*idx))%a ↦ₐ WInt (kvs_full_key user_key nkey) ∗
+              isKVS_open (cgp_b ^+ 1)%a m (idx) ∗
+              (cgp_b ^+ (1+2*idx))%a ↦ₐ WInt fkey ∗
               (cgp_b ^+ (2+2*idx))%a ↦ₐ w ∗
 
               ⌜ withinBounds cgp_b cgp_e (cgp_b ^+ (2 + 2 * idx))%a = true ⌝ ∗
@@ -290,82 +271,89 @@ Section KVS_spec.
         )
       ⊢ WP Seq (Instr Executable) {{ v, ⌜v = HaltedV⌝ → na_own logrel_nais ⊤ }})%I.
   Proof.
-    intros instrs fkey ; subst instrs.
-    iIntros (HsubBounds Hbounds_cgp Hrscratch Hridx Hkey)
+    intros instrs ; subst instrs.
+    iIntros (HsubBounds Hbounds_cgp Hcgp_bound Hrscratch Hridx Hkey)
       "(HPC & Hcgp & Hrkey & [%widx Hridx] & Hrscratch & HKVS & Hkvs_frag & Hcode & Hpost)".
-    assert ( (cgp_b ^+ 33)%a < cgp_e  )%a as Hcgp_bound by admit.
     codefrag_facts "Hcode"; rename H into Hpc_contiguous ; clear H0.
 
     (* Mov ridx 0 *)
     iInstr "Hcode".
 
     remember 0%Z as n.
-    rewrite{1} Heqn.
-    iAssert (⌜ (0 <= n <= 16)%Z ⌝)%I as "%Hn"; first (iPureIntro ; lia).
+    iAssert (⌜ (0 <= n <= SIZE_MAP)%Z ⌝)%I as "%Hn"; first (iPureIntro ; lia).
     rewrite{1} (_ : (cgp_b ^+ 1)%a = (cgp_b ^+ (1 + 2 * n))%a); last by solve_addr.
+    assert (forall i, (0 <= i < Z.to_nat n) -> ∃ (k : Z) (w : Word),  m !! i = Some (k,w) ∧ k ≠ fkey)
+    as Hfkey_notin_nfirst.
+    { rewrite Heqn; intros i Hi; lia. }
     clear Heqn.
-    (* remember (WCap RW Global cgp_b cgp_e (cgp_b ^+ (1 + 2 * n))%a) as gp. *)
-    (* clear Heqgp. *)
 
-    iLöb as "IH" forall (n Hn).
+    iLöb as "IH" forall (n Hn Hfkey_notin_nfirst).
     (* sub rscratch SIZE_MAP ridx; *)
     iDestruct "Hrscratch" as "[%wrscratch Hrscratch]".
     iInstr "Hcode".
-    destruct (decide ((16 - n) = 0)%Z) as [Hneq|Hneq].
+    replace 16 with SIZE_MAP by (by rewrite /SIZE_MAP).
+    destruct (decide ((SIZE_MAP - n) = 0)%Z) as [Hneq|Hneq].
     { (* End of the loop. It means that the key wasn't found in the KVS *)
-      (* We know that it should be a contradiction, because `(user_key, nkey)⤇(KVS) w`
+      (* We know that it should be a contradiction, because `fkey⤇(KVS) w`
          witnesses that it exists
        *)
       rewrite Hneq.
-      assert ( n = 16 ) as -> by lia.
-      (* jnz (".loop_body")%asm rscratch; *)
-      iInstr "Hcode".
-      (* jmp (".loop_end_not_found")%asm; *)
-      iInstr "Hcode".
-      (* lea cgp (-(2*SIZE_MAP))%Z; *)
-      iInstr "Hcode".
-      { transitivity (Some (cgp_b^+ 1)%a) ; solve_addr. }
-      (* mov ridx (-1)%Z; *)
-      iInstr "Hcode".
-      admit.
+      assert ( n = SIZE_MAP ) as -> by lia.
+
+      iDestruct "HKVS" as "( [%Hkvs_dom %Hkvs_uniqueness] & Hkvs_auth & HKVS)".
+      iDestruct (kvs_frag_kvs_frag_idx with "Hkvs_frag") as "(%idx & Hkvs_frag)".
+      iDestruct (gen_heap_valid with "Hkvs_auth Hkvs_frag") as "%Hm_idx".
+      exfalso.
+
+      assert (0 <= idx < SIZE_MAP) as Hidx.
+      { apply elem_of_dom_2 in Hm_idx.
+        rewrite Hkvs_dom /kvs_dom in Hm_idx.
+        apply elem_of_set_seq in Hm_idx.
+        lia.
+      }
+      apply Hfkey_notin_nfirst in Hidx as (k' & w' & Hm_idx' & Hneq_keys).
+      rewrite Hm_idx in Hm_idx'; simplify_eq.
     }
-    assert (0 ≤ n < 16)%Z as Hn' by lia.
+    assert (0 ≤ n < SIZE_MAP)%Z as Hn' by lia.
     (* jnz (".loop_body")%asm rscratch; *)
     iInstr "Hcode".
     { by injection. }
-    (* load rscratch cgp; *)
 
-    (* iDestruct (kvs_frag_kvs_frag_idx with "Hkvs_frag") as "(%idx & Hkvs_frag)". *)
-    (* iDestruct (open_isKVS_kvs_frag_idx with "[$HKVS $Hkvs_frag]") as "(HKVS & [Hbk Hbw] & Hkvs_frag)". *)
-    iDestruct (open_isKVS _ _ n with "HKVS") as "(%ku' & %kn' & %w' & HKVS & Hbk' & Hbw')"; first done.
-    replace ((cgp_b ^+ 1) ^+ 2 * n)%a  with (cgp_b ^+ (1 + 2 * n))%a by solve_addr+Hn.
-    replace ((cgp_b ^+ 1) ^+ (1 + 2 * n))%a with (cgp_b ^+ (2 + 2 * n))%a by solve_addr+Hn.
-    iInstr "Hcode".
-    { split; [done | solve_addr]. }
-
-    (* sub rscratch rkey rscratch; *)
-    iInstr "Hcode".
-    destruct (decide ( (fkey - kvs_full_key ku' kn') = 0)%Z) as [Heqfullkey | Heqfullkey].
-    - (* keys are equal *)
+    iDestruct (kvs_frag_kvs_frag_idx with "Hkvs_frag") as "(%idx & Hkvs_frag)".
+    destruct (decide (Z.of_nat idx = n)%Z) as [<- | Hneq'].
+    - iDestruct (open_isKVS_kvs_frag_idx with "[$HKVS $Hkvs_frag]") as "(HKVS & [Hbk Hbw] & Hkvs_frag)".
+      replace ((cgp_b ^+ 1) ^+ 2 * idx)%a  with (cgp_b ^+ (1 + 2 * idx))%a by solve_addr+Hn.
+      replace ((cgp_b ^+ 1) ^+ (2 * idx + 1))%a with (cgp_b ^+ (2 + 2 * idx))%a by solve_addr+Hn.
+      (* load rscratch cgp; *)
+      iInstr "Hcode".
+      { split; [done |solve_addr]. }
+      (* sub rscratch rkey rscratch; *)
+      iInstr "Hcode".
       (* jnz (".not_same_key")%asm rscratch; *)
-      rewrite Heqfullkey.
+      replace (fkey - (fkey, w).1)%Z with 0%Z by (cbn;lia).
       iInstr "Hcode".
       (* jmp (".loop_end_found")%asm; *)
       iInstr "Hcode".
 
-      assert ( (kvs_full_key user_key nkey = kvs_full_key ku' kn')%Z ) as Heqfullkey' by lia.
-      apply kvs_full_key_inj in Heqfullkey' as [<- <-].
-      {
-        assert (w' = w) as -> by admit.
-        iApply ("Hpost" $! n); iFrame.
-        iPureIntro ; split ; first lia.
-        admit.
-      }
-      all: admit.
-    - (* keys are not equal *)
+      cbn.
+      iApply "Hpost"; iFrame.
+      iPureIntro; split; first lia.
+      rewrite /withinBounds; solve_addr.
+
+    - iDestruct (open_isKVS_kvs_frag_idx_diff _ _ _ (Z.to_nat n) with "[$HKVS $Hkvs_frag]")
+        as "(%k' & %w' & %Hkk' & %Hm_idx' & HKVS  & Hkvs_frag & [Hbk Hbw])".
+      { lia. }
+      { lia. }
+      replace ((cgp_b ^+ 1) ^+ 2 * Z.to_nat n)%a  with (cgp_b ^+ (1 + 2 * n))%a by solve_addr+Hn.
+      replace ((cgp_b ^+ 1) ^+ (2 * Z.to_nat n + 1))%a with (cgp_b ^+ (2 + 2 * n))%a by solve_addr+Hn.
+      (* load rscratch cgp; *)
+      iInstr "Hcode".
+      { split; [done | solve_addr]. }
+      (* sub rscratch rkey rscratch; *)
+      iInstr "Hcode".
       (* jnz (".not_same_key")%asm rscratch; *)
       iInstr "Hcode".
-      { by injection. }
+      { injection; cbn; lia. }
       (* lea cgp 2; *)
       iInstr "Hcode".
       { transitivity (Some ( (cgp_b ^+ (1 + 2 * (n+1)))%a)); solve_addr. }
@@ -374,14 +362,21 @@ Section KVS_spec.
       (* jmp (".loop_start"); *)
       iInstr "Hcode".
       { transitivity (Some ( (pc_a ^+ 1)%a)); solve_addr. }
-      replace (cgp_b ^+ (1 + 2 * n))%a with ((cgp_b ^+ 1) ^+ 2 * n)%a by solve_addr+Hn.
-      replace (cgp_b ^+ (2 + 2 * n))%a with ((cgp_b ^+ 1) ^+ (1 + 2 * n))%a  by solve_addr+Hn.
 
-      iDestruct (close_isKVS with "[$HKVS $Hbk' $Hbw']") as "HKVS"; first done.
+      iDestruct (close_isKVS with "[$HKVS Hbk Hbw]") as "HKVS";eauto.
+      {
+        replace (cgp_b ^+ (1 + 2 * n))%a with ((cgp_b ^+ 1) ^+ 2 * Z.to_nat n)%a by solve_addr+Hn.
+        replace (cgp_b ^+ (2 + 2 * n))%a  with ((cgp_b ^+ 1) ^+ (2 * Z.to_nat n + 1))%a by solve_addr+Hn.
+        iFrame.
+      }
 
-      iApply ("IH" with "[] [$Hcgp] [$Hrkey] [$Hrscratch] [$HKVS] [$Hkvs_frag] [$Hpost] [$Hcode] [$HPC] [$Hridx]").
-      iPureIntro; lia.
-  Admitted.
+      iApply ("IH" with "[] [] [$Hcgp] [$Hrkey] [$Hrscratch] [$HKVS] [$Hkvs_frag] [$Hpost] [$Hcode] [$HPC] [$Hridx]").
+      + iPureIntro; lia.
+      + iPureIntro.
+        intros idx' Hidx'_bound.
+        destruct (decide (idx' = Z.to_nat n)%Z) as [-> | Hidx']; eauto.
+        apply Hfkey_notin_nfirst; lia.
+  Qed.
 
   Lemma KVS_read `{KVS : kvsLayout}
     (pc_b pc_b' pc_e pc_a : Addr)
@@ -422,7 +417,6 @@ Section KVS_spec.
 
       isKVS (cgp_b ^+ 1)%a m ∗
       fkey ⤇(KVS) w ∗
-
       ▷ (na_own logrel_nais ⊤ ∗
          PC ↦ᵣ updatePcPerm wret ∗
          cgp ↦ᵣ - ∗
